Fin74.lean
@@ -3,4 +3,7 @@ module  -- shake: keep-all --deprecated_module: ignore
 public import Fin74.Formula.Basic
 public import Fin74.Formula.Substitution
 public import Fin74.Kripke.Basic
+public import Fin74.Kripke.Chain
+public import Fin74.Lemma1.Basic
 public import Fin74.Logic.Basic
+public import Fin74.Logic.Shift
